Wrote first-pass mem versions of I/O functions.

progs/io_mem.c
@@ -1,0 +1,69 @@
+#include <stddef.h>
+#include <limits.h>
+#include <stdlib.h>
+
+#define EOF (-1)
+extern int getchars(unsigned char *buf);
+extern int putchars(unsigned char *buf);
+
+
+int print_intr(unsigned int i, unsigned char *buf, int j) {
+  unsigned char q,r;
+  int k = 0;
+  if (i!=0) {
+    q=i/10u;
+    r=i%10u;
+    k = print_intr(q, buf, j);
+    buf[k] = r+'0';
+  }
+  return k + 1;
+}
+
+void print_int(unsigned int i) {
+  unsigned char *buf = malloc(5);
+  if (!buf) exit(1);
+  if (i==0){
+    buf[0] = '0';
+    buf[1] = '\n';
+  }
+  else{
+    int k = print_intr(i, buf, 0);
+    buf[k] = '\n';
+  }
+  putchars(buf);
+  free(buf);
+}
+
+/* Specification:
+   reads a sequence of characters, each in the range '0'..'9';
+   after each one (and before the next one) prints a decimal
+   representation of their cumulative sum, followed by a newline.
+   When the cumulative sum >=1000, or when EOF is reached, stops.
+*/
+
+int main(void) {
+  unsigned int n, d; char c;
+  unsigned char *buf;
+  int i, j;
+
+  n=0;
+  buf = malloc(4);
+  if (!buf) exit(1);
+  i = getchars(buf);
+  while (n<1000) {
+    for(j = 0; j < i; j++){
+      c = buf[j];
+      d = ((unsigned)c)-(unsigned)'0';
+      if (d>=10) break;
+      n+=d;
+      print_int(n);
+    }
+    i = getchars(buf);
+  }
+  free(buf);
+  return 0;
+}
+
+  
+
+  
