progs/io_specs_mem.v
@@ -1,0 +1,109 @@
+Require Import VST.floyd.proofauto.
+Require Import VST.veric.juicy_extspec.
+Require Import DeepWeb.Free.Monad.Free.
+Import MonadNotations.
+Require Import DeepWeb.Free.Monad.Common.
+Require Import DeepWeb.Free.Monad.Eq.Utt.
+Import String.
+Require Import VST.progs.io_mem. (* for CompSpecs -- do we need this? *)
+
+Inductive IO_event : Type -> Type :=
+| ERead : IO_event int
+| EWrite (c : int) : IO_event unit.
+
+Definition read : itree IO_event int := embed ERead.
+
+Definition write (c : int) : itree IO_event unit := embed (EWrite c).
+
+Definition IO_itree := itree IO_event unit.
+
+Fixpoint write_list l : IO_itree :=
+  match l with
+  | nil => Ret tt
+  | c :: rest => write c ;; write_list rest
+  end.
+
+Fixpoint read_list_aux n d : itree IO_event (list int) :=
+  match n with
+  | O => Ret d
+  | S n' => x <- read ;; read_list_aux n' (x :: d)
+  end.
+
+Definition read_list n : itree IO_event (list int) := read_list_aux n [].
+
+(* We need a layer of equivalence to allow us to use the monad laws. *)
+Definition ITREE (tr : IO_itree) := EX tr' : _, !!(eq_utt tr tr') &&
+  has_ext tr'.
+
+Lemma has_ext_ITREE : forall tr, has_ext tr |-- ITREE tr.
+Proof.
+  intro; unfold ITREE.
+  Exists tr; entailer!.
+Qed.
+
+Instance CompSpecs : compspecs. make_compspecs prog. Defined.
+Definition Vprog : varspecs. mk_varspecs prog. Defined.
+
+Definition putchars_spec := DECLARE _putchars
+  WITH sh : share, buf : val, msg : list int, k : IO_itree
+  PRE [ 1%positive OF tint ]
+    PROP (readable_share sh)
+    LOCAL (temp 1%positive buf)
+    SEP (ITREE (write_list msg ;; k); data_at sh (tarray tuchar (Zlength msg)) (map Vint msg) buf)
+  POST [ tint ]
+    PROP ()
+    LOCAL (temp ret_temp (Vint (Int.repr (Zlength msg))))
+    SEP (ITREE k; data_at sh (tarray tuchar (Zlength msg)) (map Vint msg) buf).
+
+Definition getchars_spec := DECLARE _getchars
+  WITH sh : share, buf : val, len : Z, k : list int -> IO_itree
+  PRE [ ]
+    PROP (writable_share sh)
+    LOCAL ()
+    SEP (ITREE (r <- read_list (Z.to_nat len) ;; k r); data_at_ sh (tarray tuchar len) buf)
+  POST [ tint ]
+   EX msg : list int, (* for a first pass, assume it always fills the buffer *)
+    PROP ()
+    LOCAL (temp ret_temp (Vint (Int.repr len)))
+    SEP (ITREE (k msg); data_at sh (tarray tuchar len) (map Vint msg) buf).
+
+Lemma ITREE_impl : forall tr tr', eq_utt tr tr' ->
+  ITREE tr |-- ITREE tr'.
+Proof.
+  intros.
+  unfold ITREE.
+  Intros tr1; Exists tr1; entailer!.
+  etransitivity; eauto.
+  symmetry; auto.
+Qed.
+
+Lemma ITREE_ext : forall tr tr', eq_utt tr tr' ->
+  ITREE tr = ITREE tr'.
+Proof.
+  intros; apply pred_ext; apply ITREE_impl; auto.
+  symmetry; auto.
+Qed.
+
+Lemma write_list_app : forall l1 l2,
+  eq_utt (write_list (l1 ++ l2)) (write_list l1;; write_list l2).
+Proof.
+  induction l1; simpl in *; intros.
+  - rewrite ret_bind.
+    apply push_tau; reflexivity.
+  - rewrite bind_bind.
+    apply bind_mor; [reflexivity|].
+    intro; auto.
+Qed.
+
+Definition char0 : Z := 48.
+Definition newline := 10.
+
+(* Build the external specification. *)
+Definition ext_link := ext_link_prog prog.
+
+Definition IO_ext_spec :=
+  semax_ext.add_funspecs_rec
+    ext_link
+    (ok_void_spec IO_itree).(@OK_ty)
+    (ok_void_spec IO_itree).(@OK_spec)
+    [getchars_spec; putchars_spec].
